src/Language/PlutusIR/Semantics/SemanticEquivalence/CompatibilityLemmas/TyInst.v
@@ -1,0 +1,233 @@
+Require Import PlutusCert.Language.PlutusIR.
+Import NamedTerm.
+Require Import PlutusCert.Language.PlutusIR.Semantics.Dynamic.
+Require Import PlutusCert.Language.PlutusIR.Semantics.Static.
+Require Import PlutusCert.Language.PlutusIR.Semantics.SemanticEquivalence.LogicalRelation.RelationalModel.
+Require Import PlutusCert.Language.PlutusIR.Semantics.SemanticEquivalence.Monotonicity.
+
+Require Import Arith.
+
+
+Lemma msubst_TyInst : forall ss t0 T0 t',
+    msubst ss (TyInst t0 T0) t' ->
+    exists t0', msubst ss t0 t0' /\ t' = TyInst t0' T0.
+Proof.
+  induction ss.
+  - intros. 
+    inversion H. subst.
+    exists t0.
+    split. 
+    + apply msubst_nil.
+    + reflexivity. 
+  - intros.
+    inversion H. subst.
+    rename t'0 into t''.
+    inversion H2.
+    subst.
+    edestruct IHss as [t0'' Hms0']; eauto.
+    eexists.
+    split.
+    + eapply msubst_cons.
+      * apply H7.
+      * apply Hms0'.
+    + destruct Hms0'.
+      subst.
+      reflexivity.
+Qed.
+
+Lemma msubstA_TyInst : forall ss t0 T0 t',
+    msubstA ss (TyInst t0 T0) t' ->
+    exists t0', msubstA ss t0 t0' /\ t' = TyInst t0' (msubstT ss T0).
+Proof.
+  induction ss.
+  - intros. 
+    inversion H. subst.
+    exists t0.
+    split. 
+    + apply msubstA_nil.
+    + reflexivity. 
+  - intros.
+    inversion H. subst.
+    rename t'0 into t''.
+    inversion H2.
+    subst.
+    edestruct IHss as [t0'' [HmsA__t0'' Heq]]; eauto.
+    subst.
+    eexists.
+    split.
+    * eapply msubstA_cons. eauto. eauto.
+    * reflexivity. 
+Qed.
+
+Lemma inspect_eval__TyInst1 : forall t1 T j v,
+    TyInst t1 T =[j]=> v ->
+    exists j1 v1, t1 =[j1]=> v1 /\ j1 <= j.
+Proof.
+  intros.
+  inversion H. all: subst.
+  - exists j.
+    exists (Builtin IfThenElse).
+    split; auto.
+  - exists k1.
+    exists (TyAbs X K t2).
+    split; auto.
+    assert (forall a b c, a <= a + b + c). {
+      intros.
+      induction b; induction c.
+      - rewrite <- plus_n_O.
+        rewrite <- plus_n_O.
+        auto.
+      - rewrite <- plus_n_O.
+        rewrite <- plus_n_O in IHc.
+        rewrite <- plus_n_Sm.
+        auto.
+      - rewrite <- plus_n_O.
+        rewrite <- plus_n_O in IHb.
+        rewrite <- plus_n_Sm.
+        auto.
+      - rewrite <- plus_n_Sm.
+        rewrite <- plus_n_Sm.
+        rewrite plus_Sn_m.
+        rewrite <- plus_n_Sm in IHb.
+        auto.
+    }
+    apply H0.
+Qed.
+
+(*
+Lemma e : forall e,
+    RD ck rho ->
+    (mupdate ck epty) |-* T : K ->
+    Rel RC k T rho () *)
+
+Lemma compatibility_TyInst: forall Delta Gamma e e' bX K T T' S T1,
+    Delta |-* T1 : K ->
+    substituteTCA bX T1 T T' ->
+    normalise T' S ->
+    LR_logically_approximate Delta Gamma e e' (Ty_Forall bX K T) ->
+    LR_logically_approximate Delta Gamma (TyInst e T1) (TyInst e' T1) S.
+Proof.
+  intros Delta Gamma e e' bX K T T' S T1 Hkind__T1 Hstca__T' Hnorm IH_LR.
+  unfold LR_logically_approximate.
+  
+  split. {
+    eapply T_TyInst.
+    - eapply IH_LR.
+    - apply Hkind__T1.
+    - apply Hstca__T'.
+    - apply Hnorm.
+  }
+
+  split. {
+    eapply T_TyInst.
+    - eapply IH_LR.
+    - apply Hkind__T1.
+    - apply Hstca__T'.
+    - apply Hnorm.
+  }
+
+  intros k rho env env' ct ck HeqDelta HeqGamma [H_RD H_RG].
+  subst.
+
+  intros e_msa e'_msa e_ms e'_ms.
+  intros HmsA__e_msa HmsA__e'_msa Hms__e_ms Hms__e'_ms.
+
+  destruct (msubstA_TyInst _ _ _ _ HmsA__e_msa) as [eb_msa [HmsA__eb_msa Heq]].
+  destruct (msubstA_TyInst _ _ _ _ HmsA__e'_msa) as [eb'_msa [HmsA__eb'_msa Heq']].
+  subst.
+  destruct (msubst_TyInst _ _ _ _ Hms__e_ms) as [eb_ms [Hms__eb_ms Heq]].
+  destruct (msubst_TyInst _ _ _ _ Hms__e'_ms) as [eb'_ms [Hms__eb'_ms Heq']].
+  subst.
+
+  autorewrite with RC.
+  split. {
+    replace emptyContext with (@empty Kind, mupd (msyn1 rho) empty).
+    - eapply msubst_preserves_typing_1; eauto.
+      eapply msubstA_preserves_typing_1; eauto.
+      destruct IH_LR.
+      eapply T_TyInst; eauto.
+    - rewrite mupd_empty; eauto.
+  }
+  split. {
+    replace emptyContext with (@empty Kind, mupd (msyn2 rho) empty).
+    - eapply msubst_preserves_typing_2; eauto.
+      eapply msubstA_preserves_typing_2; eauto.
+      destruct IH_LR. destruct H0.
+      eapply T_TyInst; eauto.
+    - rewrite mupd_empty; eauto.
+  }
+
+  intros j Hlt__j e_f Hev__e_f.
+
+  destruct (inspect_eval__TyInst1 _ _ _ _ Hev__e_f) as [j_1 [e_f1 [Hev__e_f1 Hlt__j_1]]].
+
+  unfold LR_logically_approximate in IH_LR.
+  destruct IH_LR as [_ [_ IH]].
+  assert (IH_RC : RC k (Ty_Forall bX K T) rho eb_ms eb'_ms) by eauto.
+  
+  autorewrite with RC in IH_RC. 
+  destruct IH_RC as [_ [_ IH_RC]].
+  assert (j_1 < k) by eauto using Nat.le_lt_trans.
+  remember (IH_RC j_1 H e_f1 Hev__e_f1).
+  clear Heqe0. clear IH_RC. rename e0 into IH_RC.
+  destruct IH_RC as [e'_f1 [j'_1 [Hev__e'_f1 Hie]]].
+
+
+  assert (exists t_, e_f1 = TyAbs bX K t_) by apply skip.
+  assert (exists t_', e'_f1 = TyAbs bX K t_') by apply skip.
+  destruct H0 as [t_ Heq]. subst.
+  destruct H1 as [t_' Heq']. subst.
+
+  assert (TyAbs bX K t_ = TyAbs bX K t_) by reflexivity.
+  assert (TyAbs bX K t_' = TyAbs bX K t_') by reflexivity.
+  assert (Rel (msubstT (msyn1 rho) T1) (msubstT (msyn2 rho) T1) (fun k t1 t2 => RC k T1 rho t1 t2)). {
+    unfold Rel.
+    intros.
+    split. {
+      eapply RC_typable_empty_1; eauto.
+    }
+    split. {
+      eapply RC_typable_empty_2; eauto.
+    }
+    intros.
+    eapply RC_monotone; eauto.
+  }
+  assert (empty |-* (msubstT (msyn1 rho) T1) : K). {
+    apply skip.
+  }
+  assert (empty |-* (msubstT (msyn2 rho) T1) : K). {
+    apply skip.
+  }
+
+  assert (exists aaa, substituteA bX (msubstT (msyn1 rho) T1) t_ aaa). {
+    eapply substituteA_total.
+  }
+  assert (exists bbb, substituteA bX (msubstT (msyn2 rho) T1) t_' bbb). {
+    eapply substituteA_total.
+  }
+  destruct H5.
+  destruct H6.
+
+  remember (Hie _ _ H0 H1 _ _ _ _ _ H3 H4 H2 H5 H6).
+  clear Heqr.
+
+  assert (k - j_1 - 1 < k - j_1) by apply skip.
+  apply r in H7.
+
+  assert (exists j_2, k = j_1 + 1 + j_2) by apply skip.
+  destruct H8 as [j_2 temp].
+
+  assert (j_2 < k - j_1 - 1) by apply skip.
+  autorewrite with RC in H7.
+  destruct H7 as [_ [_ H7]].
+  assert (t_ =[j_2]=> e_f) by apply skip.
+  remember (H7 _ H8 _ H9).
+  clear Heqe0.
+  destruct e0 as [e'_f [j'_2 [Hev__e'_f HHH]]].
+  exists e'_f.
+  eexists.
+  split. {
+    eapply E_TyInst; eauto.
+    apply skip.
+  } 
+Admitted.
